%@+leo-ver=4-thin
%@+node:gcross.20090730151355.1303:@thin FancyFixedPhaseApproximation.tex
%@@language latex
\documentclass[onecolumn,amsmath,amssymb,nofootinbib,floatfix]{revtex4}

\input{notes-prelude.in}

\title{Fancy Fixed Phase Approximation}

\begin{document}

We are working with a system in a rotating reference frame and no vector potential, so as has been computed in other notes we see that

Consider the fixed phase form given by
$$\atan\paren{\frac{\sum_{K\subseteq \{1\dots N\}\atop |K|=m} \sin\paren{\sum_{k\in K} \theta_k}}{\sum_{K\subseteq \{1\dots N\}\atop |K|=m} \cos\paren{\sum_{k\in K} \theta_k}}}\equiv\frac{S}{C},
$$
where
$$
\begin{aligned}
S&:=\sum_{K\subseteq \{1\dots N\}\atop |K|=m} s(K),\\
C&:=\sum_{K\subseteq \{1\dots N\}\atop |K|=m} c(K),\\
s(K)&:=\sin\paren{\sum_{k\in K} \theta_k},\\
c(K)&:=\cos\paren{\sum_{k\in K} \theta_k}.\\
\end{aligned}
$$
Let $\partial_i$ be a shorthand for differentiating by the $i$-th angle, i.e. $\partial_i:=\pdrv{}{\theta_i}$.  Observe that
$$
\begin{aligned}
\partial_i \paren{\atan\frac{S}{C}} &= \frac{C(\partial_i S) - S(\partial_i C)}{C^2+S^2},\\
\partial_i S&:=\sum_{{K\subseteq \{1\dots N\}\atop |K|=m}\atop i\in K} c(K),\\
\partial_i C&:=\sum_{{K\subseteq \{1\dots N\}\atop |K|=m}\atop i\in K} -s(K),\\
\end{aligned}
$$
and hence,
$$
\partial_i \paren{\atan\frac{S}{C}} = \frac{\big(\sum_K c(K)\big)\big(\sum_{K',i\in K'} c(K')\big)+\big(\sum_K s(K)\big)\big(\sum_{K',i\in K'} s(K)\big)}{\big(\sum_K c(K)\big)\big(\sum_{K'} c(K)\big)+\big(\sum_K s(K)\big)\big(\sum_{K'} s(K)\big)}
$$

Recalling the trigonometric identity,
$$\cos\theta_i\cos\theta_j+\sin\theta_i\sin\theta_j,$$
we observe that the above can be rewritten in the form,
$$
\begin{aligned}
\partial_i \paren{\atan\frac{S}{C}}
&= \frac{\sum_{K,K',i\in K'}\cos\paren{\sum_{k\in K} \theta_k - \sum_{k'\in K'} \theta_{k'}}}
        {\sum_{K,K'}\cos\paren{\sum_{k\in K} \theta_k - \sum_{k'\in K'} \theta_{k'}}}\\
&= \frac{\text{Re}\left[\sum_{K,K',i\in K'}e^{i\sum_{k\in K} \theta_k-i\sum_{k'\in K'} \theta_{k'}}\right]}
        {\text{Re}\left[\sum_{K,K'}e^{i\sum_{k\in K} \theta_k-i\sum_{k'\in K'} \theta_{k'}}\right]}\\
&= \frac{\text{Re}\left[\sum_{K,K',i\in K'}\prod_{\theta\in\{\theta_k|k\in K\}\cup\{-\theta_{k'}|k'\in K'\}} e^{i\theta}\right]}
        {\text{Re}\left[\sum_{K,K'}\prod_{\theta\in\{\theta_k|k\in K\}\cup\{-\theta_{k'}|k'\in K'\}} e^{i\theta}\right]}\\
\end{aligned}
$$

\end{document}
%@-node:gcross.20090730151355.1303:@thin FancyFixedPhaseApproximation.tex
%@-leo
